cava/Cava/Arrow/ExprLoweringPreservation.v
@@ -1,0 +1,168 @@
+(****************************************************************************)
+(* Copyright 2020 The Project Oak Authors                                   *)
+(*                                                                          *)
+(* Licensed under the Apache License, Version 2.0 (the "License")           *)
+(* you may not use this file except in compliance with the License.         *)
+(* You may obtain a copy of the License at                                  *)
+(*                                                                          *)
+(*     http://www.apache.org/licenses/LICENSE-2.0                           *)
+(*                                                                          *)
+(* Unless required by applicable law or agreed to in writing, software      *)
+(* distributed under the License is distributed on an "AS IS" BASIS,        *)
+(* WITHOUT WARRANTIES OR CONDITIONS OF ANY KIND, either express or implied. *)
+(* See the License for the specific language governing permissions and      *)
+(* limitations under the License.                                           *)
+(****************************************************************************)
+
+Require Import Coq.Init.Nat.
+Require Import Coq.Lists.List.
+Require Import coqutil.Tactics.Tactics.
+Require Import Arrow.Arrow.
+Require Import Arrow.Category.
+Require Import Arrow.CircuitArrow.
+Require Import Cava.Arrow.ArrowKind.
+Require Import Cava.Arrow.CircuitProp.
+Require Import Cava.Arrow.CircuitSemantics.
+Require Import Cava.Arrow.ExprEquiv.
+Require Import Cava.Arrow.ExprLowering.
+Require Import Cava.Arrow.ExprSemantics.
+Require Import Cava.Arrow.ExprSyntax.
+
+(* TODO: this is copied from CircuitFunctionalEquivalence and extended; it
+   should be moved to a more general location *)
+Local Ltac arrowsimpl :=
+  cbn [cancell cancelr uncancell uncancelr assoc unassoc first second copy drop
+               loopr loopl swap compose id
+               CircuitCat CircuitArrow CircuitArrowSwap CircuitArrowLoop
+               CircuitArrowDrop CircuitArrowCopy arrow_category as_kind
+               Datatypes.length Nat.eqb extract_nth ].
+
+Lemma rewrite_or_default_refl A x :
+  combinational_evaluation' (rewrite_or_default A A) x = x.
+Proof.
+  induction A; cbn [rewrite_or_default] in *; arrowsimpl;
+    cbn [combinational_evaluation' fst snd]; autorewrite with vsimpl;
+      try reflexivity; [ ].
+  rewrite IHA1, IHA2; eauto using surjective_pairing.
+Qed.
+
+Definition context_entry_ok
+           (ctxt_types : list Kind)
+           (ctxt_values : denote_kind (as_kind ctxt_types))
+           (e : { t : Kind & (coq_func t * natvar t)%type})
+  : Prop :=
+  let value := fst (projT2 e) in
+  let index := snd (projT2 e) in
+  reverse_nth ctxt_types index = Some (projT1 e) /\
+  combinational_evaluation' (extract_nth ctxt_types _ index) ctxt_values = value.
+
+Lemma extend_context_entry_ok_tl ctxt_types ctxt t (x : denote_kind t) e :
+  context_entry_ok ctxt_types ctxt e ->
+  context_entry_ok (t :: ctxt_types) (x, ctxt) e.
+Proof.
+  cbv [context_entry_ok]; intros.
+  repeat match goal with
+         | x : { _ & _ } |- _ => destruct x
+         | x : _ * _ |- _ => destruct x
+         | H : _ /\ _ |- _ => destruct H
+         | _ => progress cbn [projT1 projT2 fst snd rev] in *
+         end.
+  erewrite split_lookup by eauto.
+  split; [ reflexivity | ].
+  cbn [extract_nth].
+  destruct_one_match; arrowsimpl; cbn [combinational_evaluation' fst snd];
+    subst; [ | tauto ].
+  match goal with
+  | H : reverse_nth _ (length _) = Some _ |- _ =>
+    apply lookup_upper_contra in H
+  end.
+  tauto.
+Qed.
+
+Lemma extend_context_entry_ok_hd ctxt_types ctxt t (x : denote_kind t) :
+  context_entry_ok (t :: ctxt_types) (x, ctxt) (vars _ _ (x, length ctxt_types)).
+Proof.
+  cbv [context_entry_ok]. fold as_kind denote_kind in *.
+  cbn [rev projT1 projT2 fst snd vars].
+  erewrite split_lookup by eauto.
+  split; [ reflexivity | ]. cbn [extract_nth].
+  destruct_one_match; arrowsimpl; cbn [combinational_evaluation']; [ | tauto ].
+  cbn [fst snd]. apply rewrite_or_default_refl.
+Qed.
+
+Fixpoint no_letrec {var i o} (e : kappa var i o) : Prop :=
+  match e with
+  | Var _ => True
+  | Abs f => forall v, no_letrec (f v)
+  | App f x => no_letrec f /\ no_letrec x
+  | Comp e1 e2 => no_letrec e1 /\ no_letrec e2
+  | Primitive _ => True
+  | Let x f => no_letrec x /\ forall v, no_letrec (f v)
+  | LetRec _ _ => False
+  | Id => True
+  | RemoveContext e => no_letrec e
+  end.
+Definition NoLetRec {i o} (e : Kappa i o) : Prop := no_letrec (e unitvar).
+
+Lemma no_letrec_unitvar_equiv
+      i o var (expr1 : kappa unitvar i o) (expr2 : kappa var i o) G :
+  kappa_equivalence G expr1 expr2 ->
+  no_letrec expr1 ->
+  no_letrec expr2.
+Proof.
+  induction 1; intros; cbn [no_letrec] in *; destruct_products; solve [eauto].
+  Unshelve. apply tt.
+Qed.
+
+Lemma closure_conversion'_preserves_semantics i o :
+  forall (expr1 : kappa coq_func i o) (expr2 : kappa natvar i o) G,
+    kappa_equivalence G expr1 expr2 ->
+    no_letrec expr1 ->
+    forall (ctxt_types : list Kind) (ctxt : denote_kind (as_kind ctxt_types))
+      (x : denote_kind i),
+      Forall (context_entry_ok ctxt_types ctxt) G ->
+      interp_combinational' expr1 x
+      = combinational_evaluation'
+          (closure_conversion' ctxt_types expr2) (x, ctxt).
+Proof.
+  induction 1; intros.
+  all:cbn [interp_combinational' closure_conversion'].
+  all:cbn [denote_kind no_letrec] in *; destruct_products.
+  all:arrowsimpl; cbn [combinational_evaluation' fst snd].
+  { (* Var *)
+    match goal with
+    | HForall : Forall ?P ?l, HIn : In ?x ?l |- _ =>
+      let H := fresh in
+      assert (H : P x) by (eapply Forall_forall; eauto);
+        destruct H as [? ?]
+    end.
+    cbn [vars projT1 projT2 fst snd] in *.
+    congruence. }
+  { (* Abs *)
+    match goal with
+    | IH : _ |- _ => erewrite IH with (ctxt_types:=_ :: ctxt_types)
+    end; [ reflexivity | solve [eauto] | ].
+    apply Forall_cons; [ solve [apply extend_context_entry_ok_hd] | ].
+    eapply Forall_impl; [ | eassumption].
+    apply extend_context_entry_ok_tl. }
+  { (* App *)
+    erewrite IHkappa_equivalence1, IHkappa_equivalence2 by eauto.
+    reflexivity. }
+  { (* Comp *)
+    erewrite IHkappa_equivalence1, IHkappa_equivalence2 by eauto.
+    reflexivity. }
+  { (* Primitive *) reflexivity. }
+  { (* LetRec *) tauto. }
+  { (* Id *) reflexivity. }
+Qed.
+
+Theorem closure_conversion_preserves_semantics i o (expr : Kappa i o) x :
+  Wf expr -> NoLetRec expr ->
+  interp_combinational (expr coq_func) x = combinational_evaluation
+                                             (closure_conversion expr) x.
+Proof.
+  cbv [Wf interp_combinational combinational_evaluation closure_conversion].
+  intros; arrowsimpl; cbn [combinational_evaluation'].
+  eapply closure_conversion'_preserves_semantics with (ctxt_types:=nil) (G:=nil);
+    eauto using Forall_nil, no_letrec_unitvar_equiv.
+Qed.
